ExistentialRules.lean
@@ -18,6 +18,7 @@ import ExistentialRules.ChaseSequence.ChaseTree
 import ExistentialRules.ChaseSequence.Universality
 import ExistentialRules.ChaseSequence.Deterministic
 import ExistentialRules.ChaseSequence.Nontermination.RpcLike
+import ExistentialRules.ChaseSequence.Nontermination.SparseSubderivationGenerator
 import ExistentialRules.ChaseSequence.Termination.Basic
 import ExistentialRules.ChaseSequence.Termination.BacktrackingOfFacts
 import ExistentialRules.ChaseSequence.Termination.ConstantMappings
