ExistentialRules/ChaseSequence/Nontermination/RpcLike.lean
@@ -6,6 +6,7 @@ Released under Apache 2.0 license as described in the file LICENSE.
 module
 
 public import ExistentialRules.ChaseSequence.Termination.Basic
+import ExistentialRules.ChaseSequence.Nontermination.SparseSubderivationGenerator
 
 /-!
 # RPC-like Non-Termination
@@ -112,12 +113,12 @@ theorem infinite {cd : CyclicityDerivation obs rules} : ¬ cd.terminates := by
   apply FactSet.terms_subset_of_subset (cd.facts_node_subset_of_prec (node_last node2))
   exact t_mem
 
-/-
+/-- In every `TreeDerivation`, there exists a branch that corresponds to the `CyclicityDerivation`, meaning that it has the same result. -/
 theorem corresponding_tree_branch_exists {cd : CyclicityDerivation obs rules} (td : TreeDerivation obs rules) :
     ∃ deriv ∈ td.branches, deriv.result = cd.result := by
   -- The construction is going to be annoying. The idea is to get a derivation from the "unblockable" condition, which can generate an infinite list of tree nodes for us. However, they do not directly correspond to a branch as there are big "holes" between. But we can easily fill them in by the node addresses. So the idea is clear. Only executing it will be not so nice. Maybe we can introduce some more machinery to ease the process.
+  -- TODO: this should use TreeDerivation.generate_subderivation_from_sparse_of_total_generator
   sorry
--/
 
 end CyclicityDerivation
 
@@ -130,16 +131,17 @@ structure CyclicityBranch (obs : ObsolescenceCondition sig) (kb : KnowledgeBase 
     facts_contain_origin_result := by simp
   }
 
-/-
 namespace CyclicityBranch
 
 variable {obs : ObsolescenceCondition sig} {kb : KnowledgeBase sig}
 
+/-- In every `ChaseTree`, there exists a branch that corresponds to the `CyclicityBranch`, meaning that it has the same result. -/
 theorem corresponding_tree_branch_exists {cb : CyclicityBranch obs kb} (ct : ChaseTree obs kb) :
     ∃ branch : ChaseBranch obs kb, branch.toChaseDerivation ∈ ct.branches ∧ branch.result = cb.result := by
   rcases cb.toCyclicityDerivation.corresponding_tree_branch_exists ct.toTreeDerivation with ⟨cd, cd_mem, res_eq⟩
   exists ct.chaseBranch_for_branch cd_mem
 
+/-- If a KB admist a `CyclicityBranch`, then its rule set `neverTerminates`. -/
 theorem neverTerminates_of_cyclicityBranch {obs : ObsolescenceCondition sig} {kb : KnowledgeBase sig}
     (cb : CyclicityBranch obs kb) : kb.rules.neverTerminates obs := by
   exists kb.db
@@ -151,5 +153,4 @@ theorem neverTerminates_of_cyclicityBranch {obs : ObsolescenceCondition sig} {kb
   exact terminates
 
 end CyclicityBranch
--/
 
